@prefix core:  <http://www.opengis.net/citygml/2.0/core#> .
@prefix wtr:   <http://www.opengis.net/citygml/waterbody/2.0/waterbody#> .
@prefix iso19150-2: <http://def.isotc211.org/iso19150/-2/2012/base#> .
@prefix owl:   <http://www.w3.org/2002/07/owl#> .
@prefix rdf:   <http://www.w3.org/1999/02/22-rdf-syntax-ns#> .
@prefix gsp:   <http://www.opengis.net/ont/geosparql#> .
@prefix xsd:   <http://www.w3.org/2001/XMLSchema#> .
@prefix iso19136: <http://def.isotc211.org/iso19136/2007/GML> .
@prefix skos:  <http://www.w3.org/2004/02/skos/core#> .
@prefix rdfs:  <http://www.w3.org/2000/01/rdf-schema#> .

wtr:WaterBody  a         owl:Class ;
        rdfs:label       "WaterBody"@en ;
        rdfs:subClassOf  wtr:AbstractWaterObject ;
        rdfs:subClassOf  [ a                  owl:Restriction ;
                           owl:allValuesFrom  gsp:Geometry ;
                           owl:onProperty     wtr:WaterBody.lod3Solid
                         ] ;
        rdfs:subClassOf  [ a                  owl:Restriction ;
                           owl:allValuesFrom  gsp:Geometry ;
                           owl:onProperty     wtr:WaterBody.lod1MultiSurface
                         ] ;
        rdfs:subClassOf  [ a                  owl:Restriction ;
                           owl:allValuesFrom  gsp:Geometry ;
                           owl:onProperty     wtr:WaterBody.lod1MultiCurve
                         ] ;
        rdfs:subClassOf  [ a                  owl:Restriction ;
                           owl:allValuesFrom  iso19136:Code ;
                           owl:onProperty     wtr:WaterBody.class
                         ] ;
        rdfs:subClassOf  [ a                  owl:Restriction ;
                           owl:allValuesFrom  gsp:Geometry ;
                           owl:onProperty     wtr:WaterBody.lod0MultiSurface
                         ] ;
        rdfs:subClassOf  [ a                  owl:Restriction ;
                           owl:allValuesFrom  iso19136:Code ;
                           owl:onProperty     wtr:WaterBody.function
                         ] ;
        rdfs:subClassOf  [ a                  owl:Restriction ;
                           owl:allValuesFrom  wtr:AbstractWaterBoundarySurface ;
                           owl:onProperty     wtr:WaterBody.boundedBy
                         ] ;
        rdfs:subClassOf  [ a                  owl:Restriction ;
                           owl:allValuesFrom  gsp:Geometry ;
                           owl:onProperty     wtr:WaterBody.lod1Solid
                         ] ;
        rdfs:subClassOf  [ a                  owl:Restriction ;
                           owl:allValuesFrom  gsp:Geometry ;
                           owl:onProperty     wtr:WaterBody.lod0MultiCurve
                         ] ;
        rdfs:subClassOf  [ a                  owl:Restriction ;
                           owl:allValuesFrom  gsp:Geometry ;
                           owl:onProperty     wtr:WaterBody.lod2Solid
                         ] ;
        rdfs:subClassOf  [ a                  owl:Restriction ;
                           owl:allValuesFrom  iso19136:Code ;
                           owl:onProperty     wtr:WaterBody.usage
                         ] ;
        rdfs:subClassOf  [ a                  owl:Restriction ;
                           owl:allValuesFrom  gsp:Geometry ;
                           owl:onProperty     wtr:WaterBody.lod4Solid
                         ] ;
        skos:definition  "SIG3D: Any significant accumulation of water, usually covering a part of the Earth"@en ;
        skos:prefLabel   "WaterBody"@en .

wtr:WaterBody.lod1MultiCurve
        a                owl:ObjectProperty ;
        rdfs:domain      wtr:WaterBody ;
        rdfs:label       "lod1MultiCurve"@en ;
        rdfs:range       gsp:Geometry ;
        skos:definition  "SIG3D: Relation to a LOD0 curve geometry of WaterBody.The LOD concept for module WaterBody is defined in chapter ..."@en ;
        skos:prefLabel   "lod1MultiCurve"@en .

wtr:WaterBody.usage  a   owl:ObjectProperty ;
        rdfs:domain      wtr:WaterBody ;
        rdfs:label       "usage"@en ;
        rdfs:range       iso19136:Code ;
        skos:definition  "SIG3D: Actual usage of WaterBody as given by the relevant national regulations, information communities, or specific applications."@en ;
        skos:prefLabel   "usage"@en .

wtr:WaterBody.lod1Solid
        a                owl:ObjectProperty ;
        rdfs:domain      wtr:WaterBody ;
        rdfs:label       "lod1Solid"@en ;
        rdfs:range       gsp:Geometry ;
        skos:definition  "SIG3D: Relation to a LOD1 solid geometry of WaterBody. The LOD concept for the module WaterBody is defined in chapter ..."@en ;
        skos:prefLabel   "lod1Solid"@en .

wtr:WaterClosureSurface
        a                owl:Class ;
        rdfs:label       "WaterClosureSurface"@en ;
        rdfs:subClassOf  wtr:AbstractWaterBoundarySurface ;
        skos:definition  "SIG3D: Exterior or interior boundary surface, which provides imaginary boundaries, used to describe parts of the outer shell of WaterBody."@en ;
        skos:prefLabel   "WaterClosureSurface"@en .

wtr:WaterBody.function
        a                owl:ObjectProperty ;
        rdfs:domain      wtr:WaterBody ;
        rdfs:label       "function"@en ;
        rdfs:range       iso19136:Code ;
        skos:definition  "SIG3D: Specified function of WaterBody as given by the relevant national regulations, information communities, or specific applications."@en ;
        skos:prefLabel   "function"@en .

wtr:WaterSurface  a      owl:Class ;
        rdfs:label       "WaterSurface"@en ;
        rdfs:subClassOf  wtr:AbstractWaterBoundarySurface ;
        rdfs:subClassOf  [ a                  owl:Restriction ;
                           owl:allValuesFrom  iso19136:Code ;
                           owl:onProperty     wtr:WaterSurface.waterLevel
                         ] ;
        skos:definition  "SIG3D: Exterior boundary surface of a boundary layer between water and the atmosphere, used to describe parts of the outer shell of WaterBody."@en ;
        skos:prefLabel   "WaterSurface"@en .

wtr:WaterBody.lod3Solid
        a                owl:ObjectProperty ;
        rdfs:domain      wtr:WaterBody ;
        rdfs:label       "lod3Solid"@en ;
        rdfs:range       gsp:Geometry ;
        skos:definition  "SIG3D: Relation to a LOD3 solid geometry of WaterBody. The LOD concept for the module WaterBody is defined in chapter ..."@en ;
        skos:prefLabel   "lod3Solid"@en .

wtr:AbstractWaterBoundarySurface.lod2Surface
        a                owl:ObjectProperty ;
        rdfs:domain      wtr:AbstractWaterBoundarySurface ;
        rdfs:label       "lod2Surface"@en ;
        rdfs:range       gsp:Geometry ;
        skos:definition  "SIG3D:  Relation to a LOD2 surface geometry of AbstractWaterBoundarySurface.The LOD concept for the module WaterBody is defined in chapter ..."@en ;
        skos:prefLabel   "lod2Surface"@en .

wtr:WaterBody.lod2Solid
        a                owl:ObjectProperty ;
        rdfs:domain      wtr:WaterBody ;
        rdfs:label       "lod2Solid"@en ;
        rdfs:range       gsp:Geometry ;
        skos:definition  "SIG3D: Relation to a LOD2 solid geometry of WaterBody. The LOD concept for the module WaterBody is defined in chapter ..."@en ;
        skos:prefLabel   "lod2Solid"@en .

<http://www.opengis.net/citygml/waterbody/2.0/waterbody>
        a               owl:Ontology ;
        rdfs:label      "WaterBody"@en ;
        owl:imports     <http://www.opengis.net/citygml/2.0/core> , <http://www.opengis.net/ont/geosparql> , <http://def.isotc211.org/iso19150/-2/2012/base> ;
        skos:prefLabel  "WaterBody"@en .

[ a            owl:AllDisjointClasses ;
  owl:members  ( wtr:WaterClosureSurface wtr:WaterGroundSurface wtr:WaterSurface )
] .

wtr:WaterGroundSurface
        a                owl:Class ;
        rdfs:label       "WaterGroundSurface"@en ;
        rdfs:subClassOf  wtr:AbstractWaterBoundarySurface ;
        skos:definition  "SIG3D: Exterior boundary surface of the submerged bottom of a water body, used to describe parts of the outer shell of WaterBody."@en ;
        skos:prefLabel   "WaterGroundSurface"@en .

wtr:WaterBody.lod0MultiSurface
        a                owl:ObjectProperty ;
        rdfs:domain      wtr:WaterBody ;
        rdfs:label       "lod0MultiSurface"@en ;
        rdfs:range       gsp:Geometry ;
        skos:definition  "SIG3D: Relation to a LOD0 surface geometry of WaterBody.The LOD concept for the module WaterBody is defined in chapter ..."@en ;
        skos:prefLabel   "lod0MultiSurface"@en .

wtr:AbstractWaterObject
        a                      owl:Class ;
        rdfs:label             "AbstractWaterObject"@en ;
        rdfs:subClassOf        core:AbstractCityObject ;
        iso19150-2:isAbstract  true ;
        skos:definition        "SIG3D: Abstract superclass of WaterBody."@en ;
        skos:prefLabel         "AbstractWaterObject"@en .

wtr:WaterBody.lod4Solid
        a                owl:ObjectProperty ;
        rdfs:domain      wtr:WaterBody ;
        rdfs:label       "lod4Solid"@en ;
        rdfs:range       gsp:Geometry ;
        skos:definition  "SIG3D: Relation to a LOD4 solid geometry of WaterBody. The LOD concept for the module WaterBody is defined in chapter ..."@en ;
        skos:prefLabel   "lod4Solid"@en .

wtr:WaterSurface.waterLevel
        a                owl:ObjectProperty ;
        rdfs:domain      wtr:WaterSurface ;
        rdfs:label       "waterLevel"@en ;
        rdfs:range       iso19136:Code ;
        skos:definition  "SIG3D: Codelist of the WaterSurface property waterLevel."@en ;
        skos:prefLabel   "waterLevel"@en .

wtr:AbstractWaterBoundarySurface.lod3Surface
        a                owl:ObjectProperty ;
        rdfs:domain      wtr:AbstractWaterBoundarySurface ;
        rdfs:label       "lod3Surface"@en ;
        rdfs:range       gsp:Geometry ;
        skos:definition  "SIG3D: Relation to a LOD3 surface geometry of AbstractWaterBoundarySurface The LOD concept for the module WaterBody is defined in chapter ..."@en ;
        skos:prefLabel   "lod3Surface"@en .

wtr:AbstractWaterBoundarySurface
        a                      owl:Class ;
        rdfs:label             "AbstractWaterBoundarySurface"@en ;
        rdfs:subClassOf        core:AbstractCityObject ;
        rdfs:subClassOf        [ a                  owl:Restriction ;
                                 owl:allValuesFrom  gsp:Geometry ;
                                 owl:onProperty     wtr:AbstractWaterBoundarySurface.lod4Surface
                               ] ;
        rdfs:subClassOf        [ a                  owl:Restriction ;
                                 owl:allValuesFrom  gsp:Geometry ;
                                 owl:onProperty     wtr:AbstractWaterBoundarySurface.lod3Surface
                               ] ;
        rdfs:subClassOf        [ a                  owl:Restriction ;
                                 owl:allValuesFrom  gsp:Geometry ;
                                 owl:onProperty     wtr:AbstractWaterBoundarySurface.lod2Surface
                               ] ;
        iso19150-2:isAbstract  true ;
        skos:definition        "SIG3D: Abstract superclass of boundary surfaces of WaterBody."@en ;
        skos:prefLabel         "AbstractWaterBoundarySurface"@en .

wtr:WaterBody.lod0MultiCurve
        a                owl:ObjectProperty ;
        rdfs:domain      wtr:WaterBody ;
        rdfs:label       "lod0MultiCurve"@en ;
        rdfs:range       gsp:Geometry ;
        skos:definition  "SIG3D: Relation to a LOD0 curve geometry of WaterBody.The LOD concept for module WaterBody is defined in chapter ..."@en ;
        skos:prefLabel   "lod0MultiCurve"@en .

wtr:AbstractWaterBoundarySurface.lod4Surface
        a                owl:ObjectProperty ;
        rdfs:domain      wtr:AbstractWaterBoundarySurface ;
        rdfs:label       "lod4Surface"@en ;
        rdfs:range       gsp:Geometry ;
        skos:definition  "SIG3D:  Relation to a LOD4 surface geometry of AbstractWaterBoundarySurface.The LOD concept for the module WaterBody is defined in chapter ..."@en ;
        skos:prefLabel   "lod4Surface"@en .

wtr:WaterBody.lod1MultiSurface
        a                owl:ObjectProperty ;
        rdfs:domain      wtr:WaterBody ;
        rdfs:label       "lod1MultiSurface"@en ;
        rdfs:range       gsp:Geometry ;
        skos:definition  "SIG3D: Relation to a LOD1 surface geometry of WaterBody.The LOD concept for the module WaterBody is defined in chapter ..."@en ;
        skos:prefLabel   "lod1MultiSurface"@en .

wtr:WaterBody.boundedBy
        a                owl:ObjectProperty ;
        rdfs:domain      wtr:WaterBody ;
        rdfs:label       "boundedBy"@en ;
        rdfs:range       wtr:AbstractWaterBoundarySurface ;
        skos:definition  "SIG3D: Relation between WaterBody and WaterBoundarySurface"@en ;
        skos:prefLabel   "boundedBy"@en .

wtr:WaterBody.class  a   owl:ObjectProperty ;
        rdfs:domain      wtr:WaterBody ;
        rdfs:label       "class"@en ;
        rdfs:range       iso19136:Code ;
        skos:definition  "SIG3D: Classification of WaterBody as given by the relevant national regulations, information communities, or specific applications."@en ;
        skos:prefLabel   "class"@en .
