@prefix core:  <http://www.opengis.net/citygml/3.0/core#> .
@prefix iso19150-2: <http://def.isotc211.org/iso19150/-2/2012/base#> .
@prefix owl:   <http://www.w3.org/2002/07/owl#> .
@prefix rdf:   <http://www.w3.org/1999/02/22-rdf-syntax-ns#> .
@prefix xsd:   <http://www.w3.org/2001/XMLSchema#> .
@prefix luse:  <http://www.opengis.net/citygml/landuse/3.0/landuse#> .
@prefix skos:  <http://www.w3.org/2004/02/skos/core#> .
@prefix rdfs:  <http://www.w3.org/2000/01/rdf-schema#> .

<http://www.opengis.net/citygml/landuse/3.0/landuse>
        a                owl:Ontology ;
        owl:imports      <http://www.opengis.net/citygml/3.0/core> , <http://def.isotc211.org/iso19150/-2/2012/base> ;
        skos:definition  "The LandUse module supports representation of areas of the earthâ€™s surface dedicated to a specific land use."@en ;
        skos:prefLabel   "LandUse"@en .

luse:LandUse.function
        a                owl:ObjectProperty ;
        rdfs:domain      luse:LandUse ;
        rdfs:range       owl:Class ;
        skos:definition  "Specifies the intended purposes of the LandUse."@en ;
        skos:prefLabel   "function"@en .

luse:LandUse.usage  a    owl:ObjectProperty ;
        rdfs:domain      luse:LandUse ;
        rdfs:range       owl:Class ;
        skos:definition  "Specifies the actual uses of the LandUse."@en ;
        skos:prefLabel   "usage"@en .

luse:ADEOfLandUse  a           owl:Class ;
        iso19150-2:isAbstract  true ;
        skos:definition        "ADEOfLandUse acts as a hook to define properties within an ADE that are to be added to a LandUse."@en ;
        skos:prefLabel         "ADEOfLandUse"@en .

luse:LandUse  a          owl:Class ;
        rdfs:subClassOf  core:AbstractThematicSurface ;
        rdfs:subClassOf  [ a                  owl:Restriction ;
                           owl:allValuesFrom  luse:ADEOfLandUse ;
                           owl:onProperty     luse:LandUse.adeOfLandUse
                         ] ;
        rdfs:subClassOf  [ a                  owl:Restriction ;
                           owl:allValuesFrom  owl:Class ;
                           owl:onProperty     luse:LandUse.usage
                         ] ;
        rdfs:subClassOf  [ a                  owl:Restriction ;
                           owl:allValuesFrom  owl:Class ;
                           owl:onProperty     luse:LandUse.function
                         ] ;
        rdfs:subClassOf  [ a                  owl:Restriction ;
                           owl:allValuesFrom  owl:Class ;
                           owl:onProperty     luse:LandUse.class
                         ] ;
        skos:definition  "A LandUse object is an area of the earth's surface dedicated to a specific land use or having a specific land cover with or without vegetation, such as sand, rock, mud flats, forest, or grasslands."@en ;
        skos:prefLabel   "LandUse"@en .

luse:LandUse.adeOfLandUse
        a                owl:ObjectProperty ;
        rdfs:domain      luse:LandUse ;
        rdfs:range       luse:ADEOfLandUse ;
        skos:definition  "Augments the LandUse with properties defined in an ADE."@en ;
        skos:prefLabel   "adeOfLandUse"@en .

luse:LandUse.class  a    owl:ObjectProperty ;
        rdfs:domain      luse:LandUse ;
        rdfs:range       owl:Class ;
        skos:definition  "Indicates the specific type of the LandUse."@en ;
        skos:prefLabel   "class"@en .
