@prefix core:  <http://www.opengis.net/citygml/3.0/core#> .
@prefix iso19150-2: <http://def.isotc211.org/iso19150/-2/2012/base#> .
@prefix iso19107: <http://def.isotc211.org/iso19107/2003/Geometry#> .
@prefix owl:   <http://www.w3.org/2002/07/owl#> .
@prefix rdf:   <http://www.w3.org/1999/02/22-rdf-syntax-ns#> .
@prefix gsp:   <http://www.opengis.net/ont/geosparql#> .
@prefix xsd:   <http://www.w3.org/2001/XMLSchema#> .
@prefix skos:  <http://www.w3.org/2004/02/skos/core#> .
@prefix rdfs:  <http://www.w3.org/2000/01/rdf-schema#> .
@prefix iso19123: <http://def.isotc211.org/iso19123/2005/Coverages> .
@prefix dem:   <http://www.opengis.net/citygml/relief/3.0/relief#> .

dem:MassPointRelief.reliefPoints
        a                owl:ObjectProperty ;
        rdfs:domain      dem:MassPointRelief ;
        rdfs:range       gsp:Geometry ;
        skos:definition  "Relates to the 3D MultiPoint geometry of the MassPointRelief."@en ;
        skos:prefLabel   "reliefPoints"@en .

dem:AbstractReliefComponent
        a                      owl:Class ;
        rdfs:subClassOf        core:AbstractSpaceBoundary ;
        rdfs:subClassOf        [ a                  owl:Restriction ;
                                 owl:allValuesFrom  dem:ADEOfAbstractReliefComponent ;
                                 owl:onProperty     dem:AbstractReliefComponent.adeOfAbstractReliefComponent
                               ] ;
        rdfs:subClassOf        [ a                  owl:Restriction ;
                                 owl:allValuesFrom  gsp:Geometry ;
                                 owl:onProperty     dem:AbstractReliefComponent.extent
                               ] ;
        rdfs:subClassOf        [ a                  owl:Restriction ;
                                 owl:allValuesFrom  core:IntegerBetween0and3 ;
                                 owl:onProperty     dem:AbstractReliefComponent.lod
                               ] ;
        iso19150-2:isAbstract  true ;
        skos:definition        "An AbstractReliefComponent represents an element of the terrain surface - either a TIN, a Grid, mass points or break lines."@en ;
        skos:prefLabel         "AbstractReliefComponent"@en .

dem:TINRelief.adeOfTINRelief
        a                owl:ObjectProperty ;
        rdfs:domain      dem:TINRelief ;
        rdfs:range       dem:ADEOfTINRelief ;
        skos:definition  "Augments the TINRelief with properties defined in an ADE."@en ;
        skos:prefLabel   "adeOfTINRelief"@en .

dem:ADEOfReliefFeature
        a                      owl:Class ;
        iso19150-2:isAbstract  true ;
        skos:definition        "ADEOfReliefFeature acts as a hook to define properties within an ADE that are to be added to a ReliefFeature."@en ;
        skos:prefLabel         "ADEOfReliefFeature"@en .

dem:ADEOfRasterRelief
        a                      owl:Class ;
        iso19150-2:isAbstract  true ;
        skos:definition        "ADEOfRasterRelief acts as a hook to define properties within an ADE that are to be added to a RasterRelief."@en ;
        skos:prefLabel         "ADEOfRasterRelief"@en .

dem:BreaklineRelief.ridgeOrValleyLines
        a                owl:ObjectProperty ;
        rdfs:domain      dem:BreaklineRelief ;
        rdfs:range       gsp:Geometry ;
        skos:definition  "Relates to the 3D MultiCurve geometry of the MassPointRelief. This association role is used to represent ridge or valley lines."@en ;
        skos:prefLabel   "ridgeOrValleyLines"@en .

dem:TINRelief.tin  a     owl:ObjectProperty ;
        rdfs:domain      dem:TINRelief ;
        rdfs:range       iso19107:GM_TriangulatedSurface ;
        skos:definition  "Relates to the triangulated surface of the TINRelief."@en ;
        skos:prefLabel   "tin"@en .

dem:BreaklineRelief  a   owl:Class ;
        rdfs:subClassOf  dem:AbstractReliefComponent ;
        rdfs:subClassOf  [ a                  owl:Restriction ;
                           owl:allValuesFrom  dem:ADEOfBreaklineRelief ;
                           owl:onProperty     dem:BreaklineRelief.adeOfBreaklineRelief
                         ] ;
        rdfs:subClassOf  [ a                  owl:Restriction ;
                           owl:allValuesFrom  gsp:Geometry ;
                           owl:onProperty     dem:BreaklineRelief.breaklines
                         ] ;
        rdfs:subClassOf  [ a                  owl:Restriction ;
                           owl:allValuesFrom  gsp:Geometry ;
                           owl:onProperty     dem:BreaklineRelief.ridgeOrValleyLines
                         ] ;
        skos:definition  "A BreaklineRelief represents a terrain component with 3D lines. These lines denote break lines or ridge/valley lines."@en ;
        skos:prefLabel   "BreaklineRelief"@en .

dem:AbstractReliefComponent.lod
        a                owl:ObjectProperty ;
        rdfs:domain      dem:AbstractReliefComponent ;
        rdfs:range       core:IntegerBetween0and3 ;
        skos:definition  "Indicates the Level of Detail of the terrain component."@en ;
        skos:prefLabel   "lod"@en .

dem:AbstractReliefComponent.extent
        a                owl:ObjectProperty ;
        rdfs:domain      dem:AbstractReliefComponent ;
        rdfs:range       gsp:Geometry ;
        skos:definition  "Indicates the geometrical extent of the terrain component. The geometrical extent is provided as a 2D Surface geometry."@en ;
        skos:prefLabel   "extent"@en .

dem:ADEOfAbstractReliefComponent
        a                      owl:Class ;
        iso19150-2:isAbstract  true ;
        skos:definition        "ADEOfAbstractReliefComponent acts as a hook to define properties within an ADE that are to be added to AbstractReliefComponent."@en ;
        skos:prefLabel         "ADEOfAbstractReliefComponent"@en .

dem:ADEOfBreaklineRelief
        a                      owl:Class ;
        iso19150-2:isAbstract  true ;
        skos:definition        "ADEOfBreaklineRelief acts as a hook to define properties within an ADE that are to be added to a BreaklineRelief."@en ;
        skos:prefLabel         "ADEOfBreaklineRelief"@en .

dem:MassPointRelief  a   owl:Class ;
        rdfs:subClassOf  dem:AbstractReliefComponent ;
        rdfs:subClassOf  [ a                  owl:Restriction ;
                           owl:allValuesFrom  dem:ADEOfMassPointRelief ;
                           owl:onProperty     dem:MassPointRelief.adeOfMassPointRelief
                         ] ;
        rdfs:subClassOf  [ a                  owl:Restriction ;
                           owl:allValuesFrom  core:AbstractPointCloud ;
                           owl:onProperty     dem:MassPointRelief.pointCloud
                         ] ;
        rdfs:subClassOf  [ a                  owl:Restriction ;
                           owl:allValuesFrom  gsp:Geometry ;
                           owl:onProperty     dem:MassPointRelief.reliefPoints
                         ] ;
        skos:definition  "A MassPointRelief represents a terrain component as a collection of 3D points."@en ;
        skos:prefLabel   "MassPointRelief"@en .

dem:MassPointRelief.adeOfMassPointRelief
        a                owl:ObjectProperty ;
        rdfs:domain      dem:MassPointRelief ;
        rdfs:range       dem:ADEOfMassPointRelief ;
        skos:definition  "Augments the MassPointRelief with properties defined in an ADE."@en ;
        skos:prefLabel   "adeOfMassPointRelief"@en .

dem:BreaklineRelief.adeOfBreaklineRelief
        a                owl:ObjectProperty ;
        rdfs:domain      dem:BreaklineRelief ;
        rdfs:range       dem:ADEOfBreaklineRelief ;
        skos:definition  "Augments the BreaklineRelief with properties defined in an ADE."@en ;
        skos:prefLabel   "adeOfBreaklineRelief"@en .

dem:AbstractReliefComponent.adeOfAbstractReliefComponent
        a                owl:ObjectProperty ;
        rdfs:domain      dem:AbstractReliefComponent ;
        rdfs:range       dem:ADEOfAbstractReliefComponent ;
        skos:definition  "Augments AbstractReliefComponent with properties defined in an ADE."@en ;
        skos:prefLabel   "adeOfAbstractReliefComponent"@en .

dem:ADEOfTINRelief  a          owl:Class ;
        iso19150-2:isAbstract  true ;
        skos:definition        "ADEOfTINRelief acts as a hook to define properties within an ADE that are to be added to a TINRelief."@en ;
        skos:prefLabel         "ADEOfTINRelief"@en .

dem:MassPointRelief.pointCloud
        a                owl:ObjectProperty ;
        rdfs:domain      dem:MassPointRelief ;
        rdfs:range       core:AbstractPointCloud ;
        skos:definition  "Relates to the 3D PointCloud of the MassPointRelief."@en ;
        skos:prefLabel   "pointCloud"@en .

dem:ReliefFeature.reliefComponent
        a                owl:ObjectProperty ;
        rdfs:domain      dem:ReliefFeature ;
        rdfs:range       dem:AbstractReliefComponent ;
        skos:definition  "Relates to the terrain components that are part of the ReliefFeature."@en ;
        skos:prefLabel   "reliefComponent"@en .

<http://www.opengis.net/citygml/relief/3.0/relief>
        a                owl:Ontology ;
        owl:imports      <http://www.opengis.net/ont/geosparql> , <http://www.opengis.net/citygml/3.0/core> , <http://def.isotc211.org/iso19150/-2/2012/base> ;
        skos:definition  "The Relief module supports representation of the terrain. CityGML supports terrain representations at different levels of detail, reflecting different accuracies or resolutions. Terrain may be specified as a regular raster or grid, as a TIN, by break lines, and/or by mass points."@en ;
        skos:prefLabel   "Relief"@en .

dem:ReliefFeature.lod
        a                owl:ObjectProperty ;
        rdfs:domain      dem:ReliefFeature ;
        rdfs:range       core:IntegerBetween0and3 ;
        skos:definition  "Indicates the Level of Detail of the ReliefFeature."@en ;
        skos:prefLabel   "lod"@en .

dem:ReliefFeature.adeOfReliefFeature
        a                owl:ObjectProperty ;
        rdfs:domain      dem:ReliefFeature ;
        rdfs:range       dem:ADEOfReliefFeature ;
        skos:definition  "Augments the ReliefFeature with properties defined in an ADE."@en ;
        skos:prefLabel   "adeOfReliefFeature"@en .

dem:TINRelief  a         owl:Class ;
        rdfs:subClassOf  dem:AbstractReliefComponent ;
        rdfs:subClassOf  [ a                  owl:Restriction ;
                           owl:allValuesFrom  dem:ADEOfTINRelief ;
                           owl:onProperty     dem:TINRelief.adeOfTINRelief
                         ] ;
        rdfs:subClassOf  [ a                  owl:Restriction ;
                           owl:allValuesFrom  iso19107:GM_TriangulatedSurface ;
                           owl:onProperty     dem:TINRelief.tin
                         ] ;
        skos:definition  "A TINRelief represents a terrain component as a triangulated irregular network."@en ;
        skos:prefLabel   "TINRelief"@en .

dem:RasterRelief.adeOfRasterRelief
        a                owl:ObjectProperty ;
        rdfs:domain      dem:RasterRelief ;
        rdfs:range       dem:ADEOfRasterRelief ;
        skos:definition  "Augments the RasterRelief with properties defined in an ADE."@en ;
        skos:prefLabel   "adeOfRasterRelief"@en .

dem:ReliefFeature  a     owl:Class ;
        rdfs:subClassOf  core:AbstractSpaceBoundary ;
        rdfs:subClassOf  [ a                  owl:Restriction ;
                           owl:allValuesFrom  dem:ADEOfReliefFeature ;
                           owl:onProperty     dem:ReliefFeature.adeOfReliefFeature
                         ] ;
        rdfs:subClassOf  [ a                  owl:Restriction ;
                           owl:allValuesFrom  dem:AbstractReliefComponent ;
                           owl:onProperty     dem:ReliefFeature.reliefComponent
                         ] ;
        rdfs:subClassOf  [ a                  owl:Restriction ;
                           owl:allValuesFrom  core:IntegerBetween0and3 ;
                           owl:onProperty     dem:ReliefFeature.lod
                         ] ;
        skos:definition  "A ReliefFeature is a collection of terrain components representing the Earth's surface, a.k.a. the Digital Terrain Model."@en ;
        skos:prefLabel   "ReliefFeature"@en .

[ a            owl:AllDisjointClasses ;
  owl:members  ( dem:BreaklineRelief dem:MassPointRelief dem:RasterRelief dem:TINRelief )
] .

dem:ADEOfMassPointRelief
        a                      owl:Class ;
        iso19150-2:isAbstract  true ;
        skos:definition        "ADEOfMassPointRelief acts as a hook to define properties within an ADE that are to be added to a MassPointRelief."@en ;
        skos:prefLabel         "ADEOfMassPointRelief"@en .

dem:BreaklineRelief.breaklines
        a                owl:ObjectProperty ;
        rdfs:domain      dem:BreaklineRelief ;
        rdfs:range       gsp:Geometry ;
        skos:definition  "Relates to the 3D MultiCurve geometry of the MassPointRelief. This association role is used to represent break lines."@en ;
        skos:prefLabel   "breaklines"@en .

dem:RasterRelief  a      owl:Class ;
        rdfs:subClassOf  dem:AbstractReliefComponent ;
        rdfs:subClassOf  [ a                  owl:Restriction ;
                           owl:allValuesFrom  dem:ADEOfRasterRelief ;
                           owl:onProperty     dem:RasterRelief.adeOfRasterRelief
                         ] ;
        rdfs:subClassOf  [ a                  owl:Restriction ;
                           owl:allValuesFrom  iso19123:CV_DiscreteGridPointCoverage ;
                           owl:onProperty     dem:RasterRelief.grid
                         ] ;
        skos:definition  "A RasterRelief represents a terrain component as a regular raster or grid."@en ;
        skos:prefLabel   "RasterRelief"@en .

dem:RasterRelief.grid
        a                owl:ObjectProperty ;
        rdfs:domain      dem:RasterRelief ;
        rdfs:range       iso19123:CV_DiscreteGridPointCoverage ;
        skos:definition  "Relates to the DiscreteGridPointCoverage of the RasterRelief."@en ;
        skos:prefLabel   "grid"@en .
