@prefix core:  <http://www.opengis.net/citygml/3.0/core#> .
@prefix iso19150-2: <http://def.isotc211.org/iso19150/-2/2012/base#> .
@prefix owl:   <http://www.w3.org/2002/07/owl#> .
@prefix rdf:   <http://www.w3.org/1999/02/22-rdf-syntax-ns#> .
@prefix gsp:   <http://www.opengis.net/ont/geosparql#> .
@prefix xsd:   <http://www.w3.org/2001/XMLSchema#> .
@prefix pcl:   <http://www.opengis.net/citygml/pointcloud/3.0/pointcloud#> .
@prefix skos:  <http://www.w3.org/2004/02/skos/core#> .
@prefix rdfs:  <http://www.w3.org/2000/01/rdf-schema#> .

pcl:PointCloud.pointFile
        a                owl:DatatypeProperty ;
        rdfs:domain      pcl:PointCloud ;
        rdfs:range       xsd:anyURI ;
        skos:definition  "Specifies the URI that points to the external point cloud file."@en ;
        skos:prefLabel   "pointFile"@en .

<http://www.opengis.net/citygml/pointcloud/3.0/pointcloud>
        a                owl:Ontology ;
        owl:imports      <http://www.opengis.net/ont/geosparql> , <http://www.opengis.net/citygml/3.0/core> , <http://def.isotc211.org/iso19150/-2/2012/base> ;
        skos:definition  "The PointCloud module supports representation of CityGML features by a collection of points."@en ;
        skos:prefLabel   "PointCloud"@en .

pcl:PointCloud.points
        a                owl:ObjectProperty ;
        rdfs:domain      pcl:PointCloud ;
        rdfs:range       gsp:Geometry ;
        skos:definition  "Relates to the 3D MultiPoint geometry of the PointCloud stored inline with the city model."@en ;
        skos:prefLabel   "points"@en .

pcl:PointCloud  a        owl:Class ;
        rdfs:subClassOf  core:AbstractPointCloud ;
        rdfs:subClassOf  [ a                  owl:Restriction ;
                           owl:allValuesFrom  pcl:ADEOfPointCloud ;
                           owl:onProperty     pcl:PointCloud.adeOfPointCloud
                         ] ;
        rdfs:subClassOf  [ a                  owl:Restriction ;
                           owl:allValuesFrom  gsp:Geometry ;
                           owl:onProperty     pcl:PointCloud.points
                         ] ;
        rdfs:subClassOf  [ a                  owl:Restriction ;
                           owl:allValuesFrom  xsd:string ;
                           owl:onProperty     pcl:PointCloud.pointFileSrsName
                         ] ;
        rdfs:subClassOf  [ a                  owl:Restriction ;
                           owl:allValuesFrom  xsd:anyURI ;
                           owl:onProperty     pcl:PointCloud.pointFile
                         ] ;
        rdfs:subClassOf  [ a                  owl:Restriction ;
                           owl:allValuesFrom  owl:Class ;
                           owl:onProperty     pcl:PointCloud.mimeType
                         ] ;
        skos:definition  "A PointCloud is an unordered collection of points that is a sampling of the geometry of a space or space boundary."@en ;
        skos:prefLabel   "PointCloud"@en .

pcl:PointCloud.pointFileSrsName
        a                owl:DatatypeProperty ;
        rdfs:domain      pcl:PointCloud ;
        rdfs:range       xsd:string ;
        skos:definition  "Indicates the coordinate reference system used by the external point cloud file."@en ;
        skos:prefLabel   "pointFileSrsName"@en .

pcl:PointCloud.mimeType
        a                owl:ObjectProperty ;
        rdfs:domain      pcl:PointCloud ;
        rdfs:range       owl:Class ;
        skos:definition  "Specifies the MIME type of the external point cloud file."@en ;
        skos:prefLabel   "mimeType"@en .

pcl:PointCloud.adeOfPointCloud
        a                owl:ObjectProperty ;
        rdfs:domain      pcl:PointCloud ;
        rdfs:range       pcl:ADEOfPointCloud ;
        skos:definition  "Augments the PointCloud with properties defined in an ADE."@en ;
        skos:prefLabel   "adeOfPointCloud"@en .

pcl:ADEOfPointCloud  a         owl:Class ;
        iso19150-2:isAbstract  true ;
        skos:definition        "ADEOfPointCloud acts as a hook to define properties within an ADE that are to be added to a PointCloud."@en ;
        skos:prefLabel         "ADEOfPointCloud"@en .
