@prefix sc:    <http://shapechange.net/resources/ont/base#> .
@prefix core:  <http://www.opengis.net/citygml/2.0/core#> .
@prefix iso19150-2: <http://def.isotc211.org/iso19150/-2/2012/base#> .
@prefix owl:   <http://www.w3.org/2002/07/owl#> .
@prefix rdf:   <http://www.w3.org/1999/02/22-rdf-syntax-ns#> .
@prefix gsp:   <http://www.opengis.net/ont/geosparql#> .
@prefix xsd:   <http://www.w3.org/2001/XMLSchema#> .
@prefix iso19136: <http://def.isotc211.org/iso19136/2007/GML> .
@prefix veg:   <http://www.opengis.net/citygml/vegetation/2.0/vegetation#> .
@prefix skos:  <http://www.w3.org/2004/02/skos/core#> .
@prefix rdfs:  <http://www.w3.org/2000/01/rdf-schema#> .

veg:SolitaryVegetationObject
        a                owl:Class ;
        rdfs:label       "SolitaryVegetationObject"@en ;
        rdfs:subClassOf  veg:AbstractVegetationObject ;
        rdfs:subClassOf  [ a                  owl:Restriction ;
                           owl:allValuesFrom  core:ImplicitGeometry ;
                           owl:onProperty     veg:SolitaryVegetationObject.lod3ImplicitRepresentation
                         ] ;
        rdfs:subClassOf  [ a                  owl:Restriction ;
                           owl:allValuesFrom  gsp:Geometry ;
                           owl:onProperty     veg:SolitaryVegetationObject.lod4Geometry
                         ] ;
        rdfs:subClassOf  [ a                  owl:Restriction ;
                           owl:allValuesFrom  sc:Measure ;
                           owl:onProperty     veg:SolitaryVegetationObject.crownDiameter
                         ] ;
        rdfs:subClassOf  [ a                  owl:Restriction ;
                           owl:allValuesFrom  sc:Measure ;
                           owl:onProperty     veg:SolitaryVegetationObject.trunkDiameter
                         ] ;
        rdfs:subClassOf  [ a                  owl:Restriction ;
                           owl:allValuesFrom  gsp:Geometry ;
                           owl:onProperty     veg:SolitaryVegetationObject.lod2Geometry
                         ] ;
        rdfs:subClassOf  [ a                  owl:Restriction ;
                           owl:allValuesFrom  iso19136:Code ;
                           owl:onProperty     veg:SolitaryVegetationObject.function
                         ] ;
        rdfs:subClassOf  [ a                  owl:Restriction ;
                           owl:allValuesFrom  iso19136:Code ;
                           owl:onProperty     veg:SolitaryVegetationObject.species
                         ] ;
        rdfs:subClassOf  [ a                  owl:Restriction ;
                           owl:allValuesFrom  sc:Measure ;
                           owl:onProperty     veg:SolitaryVegetationObject.height
                         ] ;
        rdfs:subClassOf  [ a                  owl:Restriction ;
                           owl:allValuesFrom  core:ImplicitGeometry ;
                           owl:onProperty     veg:SolitaryVegetationObject.lod1ImplicitRepresentation
                         ] ;
        rdfs:subClassOf  [ a                  owl:Restriction ;
                           owl:allValuesFrom  iso19136:Code ;
                           owl:onProperty     veg:SolitaryVegetationObject.usage
                         ] ;
        rdfs:subClassOf  [ a                  owl:Restriction ;
                           owl:allValuesFrom  gsp:Geometry ;
                           owl:onProperty     veg:SolitaryVegetationObject.lod1Geometry
                         ] ;
        rdfs:subClassOf  [ a                  owl:Restriction ;
                           owl:allValuesFrom  gsp:Geometry ;
                           owl:onProperty     veg:SolitaryVegetationObject.lod3Geometry
                         ] ;
        rdfs:subClassOf  [ a                  owl:Restriction ;
                           owl:allValuesFrom  core:ImplicitGeometry ;
                           owl:onProperty     veg:SolitaryVegetationObject.lod4ImplicitRepresentation
                         ] ;
        rdfs:subClassOf  [ a                  owl:Restriction ;
                           owl:allValuesFrom  iso19136:Code ;
                           owl:onProperty     veg:SolitaryVegetationObject.class
                         ] ;
        rdfs:subClassOf  [ a                  owl:Restriction ;
                           owl:allValuesFrom  core:ImplicitGeometry ;
                           owl:onProperty     veg:SolitaryVegetationObject.lod2ImplicitRepresentation
                         ] ;
        skos:definition  "SIG3D: Single vegetation object"@en ;
        skos:prefLabel   "SolitaryVegetationObject"@en .

veg:PlantCover.lod4MultiSurface
        a                owl:ObjectProperty ;
        rdfs:domain      veg:PlantCover ;
        rdfs:label       "lod4MultiSurface"@en ;
        rdfs:range       gsp:Geometry ;
        skos:definition  "SIG3D: Relation to a LOD4 surface geometry of PlantCover.The LOD concept for the module Vegetation is defined in chapter ..."@en ;
        skos:prefLabel   "lod4MultiSurface"@en .

veg:PlantCover.lod2MultiSolid
        a                owl:ObjectProperty ;
        rdfs:domain      veg:PlantCover ;
        rdfs:label       "lod2MultiSolid"@en ;
        rdfs:range       gsp:Geometry ;
        skos:definition  "SIG3D: Relation to a LOD2 multiple solid geometry of PlantCover.The LOD concept for the module Vegetation is defined in chapter ..."@en ;
        skos:prefLabel   "lod2MultiSolid"@en .

veg:PlantCover.function
        a                owl:ObjectProperty ;
        rdfs:domain      veg:PlantCover ;
        rdfs:label       "function"@en ;
        rdfs:range       iso19136:Code ;
        skos:definition  "SIG3D: Function of PlantCover as given by the relevant national regulations, information communities, or specific applications."@en ;
        skos:prefLabel   "function"@en .

veg:PlantCover  a         owl:Class ;
        rdfs:label        "PlantCover"@en ;
        rdfs:subClassOf   veg:AbstractVegetationObject ;
        rdfs:subClassOf   [ a                  owl:Restriction ;
                            owl:allValuesFrom  gsp:Geometry ;
                            owl:onProperty     veg:PlantCover.lod1MultiSolid
                          ] ;
        rdfs:subClassOf   [ a                  owl:Restriction ;
                            owl:allValuesFrom  gsp:Geometry ;
                            owl:onProperty     veg:PlantCover.lod2MultiSolid
                          ] ;
        rdfs:subClassOf   [ a                  owl:Restriction ;
                            owl:allValuesFrom  iso19136:Code ;
                            owl:onProperty     veg:PlantCover.function
                          ] ;
        rdfs:subClassOf   [ a                  owl:Restriction ;
                            owl:allValuesFrom  gsp:Geometry ;
                            owl:onProperty     veg:PlantCover.lod3MultiSolid
                          ] ;
        rdfs:subClassOf   [ a                  owl:Restriction ;
                            owl:allValuesFrom  gsp:Geometry ;
                            owl:onProperty     veg:PlantCover.lod2MultiSurface
                          ] ;
        rdfs:subClassOf   [ a                  owl:Restriction ;
                            owl:allValuesFrom  iso19136:Code ;
                            owl:onProperty     veg:PlantCover.class
                          ] ;
        rdfs:subClassOf   [ a                  owl:Restriction ;
                            owl:allValuesFrom  gsp:Geometry ;
                            owl:onProperty     veg:PlantCover.lod4MultiSurface
                          ] ;
        rdfs:subClassOf   [ a                  owl:Restriction ;
                            owl:allValuesFrom  gsp:Geometry ;
                            owl:onProperty     veg:PlantCover.lod1MultiSurface
                          ] ;
        rdfs:subClassOf   [ a                  owl:Restriction ;
                            owl:allValuesFrom  sc:Measure ;
                            owl:onProperty     veg:PlantCover.averageHeight
                          ] ;
        rdfs:subClassOf   [ a                  owl:Restriction ;
                            owl:allValuesFrom  gsp:Geometry ;
                            owl:onProperty     veg:PlantCover.lod3MultiSurface
                          ] ;
        rdfs:subClassOf   [ a                  owl:Restriction ;
                            owl:allValuesFrom  gsp:Geometry ;
                            owl:onProperty     veg:PlantCover.lod4MultiSolid
                          ] ;
        rdfs:subClassOf   [ a                  owl:Restriction ;
                            owl:allValuesFrom  iso19136:Code ;
                            owl:onProperty     veg:PlantCover.usage
                          ] ;
        owl:disjointWith  veg:SolitaryVegetationObject ;
        skos:definition   "SIG3D: Area filled with a specific vegetation"@en ;
        skos:prefLabel    "PlantCover"@en .

veg:SolitaryVegetationObject.lod4Geometry
        a                owl:ObjectProperty ;
        rdfs:domain      veg:SolitaryVegetationObject ;
        rdfs:label       "lod4Geometry"@en ;
        rdfs:range       gsp:Geometry ;
        skos:definition  "SIG3D: Relation to LOD4 geometry of SolitaryVegetationObject.The LOD concept for the module Vegetation is defined in chapter ..."@en ;
        skos:prefLabel   "lod4Geometry"@en .

veg:PlantCover.averageHeight
        a                owl:DatatypeProperty ;
        rdfs:domain      veg:PlantCover ;
        rdfs:label       "averageHeight"@en ;
        rdfs:range       sc:Measure ;
        skos:definition  "SIG3D: Average value of the heights of the grown-up plants"@en ;
        skos:prefLabel   "averageHeight"@en .

veg:PlantCover.lod4MultiSolid
        a                owl:ObjectProperty ;
        rdfs:domain      veg:PlantCover ;
        rdfs:label       "lod4MultiSolid"@en ;
        rdfs:range       gsp:Geometry ;
        skos:definition  "SIG3D: Relation to a LOD4 multiple solid geometry of PlantCover.The LOD concept for the module Vegetation is defined in chapter ..."@en ;
        skos:prefLabel   "lod4MultiSolid"@en .

veg:SolitaryVegetationObject.lod1ImplicitRepresentation
        a                owl:ObjectProperty ;
        rdfs:domain      veg:SolitaryVegetationObject ;
        rdfs:label       "lod1ImplicitRepresentation"@en ;
        rdfs:range       core:ImplicitGeometry ;
        skos:definition  "SIG3D: Relation to LOD1 implicit geometry of SolitaryVegetationObject.The LOD concept for the module Vegetation is defined in chapter ..."@en ;
        skos:prefLabel   "lod1ImplicitRepresentation"@en .

veg:SolitaryVegetationObject.lod2ImplicitRepresentation
        a                owl:ObjectProperty ;
        rdfs:domain      veg:SolitaryVegetationObject ;
        rdfs:label       "lod2ImplicitRepresentation"@en ;
        rdfs:range       core:ImplicitGeometry ;
        skos:definition  "SIG3D: Relation to LOD2 implicit geometry of SolitaryVegetationObject.The LOD concept for the module Vegetation is defined in chapter ..."@en ;
        skos:prefLabel   "lod2ImplicitRepresentation"@en .

veg:SolitaryVegetationObject.lod3ImplicitRepresentation
        a                owl:ObjectProperty ;
        rdfs:domain      veg:SolitaryVegetationObject ;
        rdfs:label       "lod3ImplicitRepresentation"@en ;
        rdfs:range       core:ImplicitGeometry ;
        skos:definition  "SIG3D: Relation to LOD3 implicit geometry of SolitaryVegetationObject.The LOD concept for the module Vegetation is defined in chapter ..."@en ;
        skos:prefLabel   "lod3ImplicitRepresentation"@en .

veg:SolitaryVegetationObject.lod4ImplicitRepresentation
        a                owl:ObjectProperty ;
        rdfs:domain      veg:SolitaryVegetationObject ;
        rdfs:label       "lod4ImplicitRepresentation"@en ;
        rdfs:range       core:ImplicitGeometry ;
        skos:definition  "SIG3D: Relation to LOD4 implicit geometry of SolitaryVegetationObject.The LOD concept for the module Vegetation is defined in chapter ..."@en ;
        skos:prefLabel   "lod4ImplicitRepresentation"@en .

veg:PlantCover.lod3MultiSolid
        a                owl:ObjectProperty ;
        rdfs:domain      veg:PlantCover ;
        rdfs:label       "lod3MultiSolid"@en ;
        rdfs:range       gsp:Geometry ;
        skos:definition  "SIG3D: Relation to a LOD3 multiple solid geometry of PlantCover.The LOD concept for the module Vegetation is defined in chapter ..."@en ;
        skos:prefLabel   "lod3MultiSolid"@en .

veg:SolitaryVegetationObject.lod1Geometry
        a                owl:ObjectProperty ;
        rdfs:domain      veg:SolitaryVegetationObject ;
        rdfs:label       "lod1Geometry"@en ;
        rdfs:range       gsp:Geometry ;
        skos:definition  "SIG3D: Relation to LOD1 geometry of SolitaryVegetationObject.The LOD concept for the module Vegetation is defined in chapter ..."@en ;
        skos:prefLabel   "lod1Geometry"@en .

veg:PlantCover.class  a  owl:ObjectProperty ;
        rdfs:domain      veg:PlantCover ;
        rdfs:label       "class"@en ;
        rdfs:range       iso19136:Code ;
        skos:definition  "SIG3D: Classification of PlantCover as given by the relevant national regulations, information communities, or specific applications."@en ;
        skos:prefLabel   "class"@en .

veg:SolitaryVegetationObject.species
        a                owl:ObjectProperty ;
        rdfs:domain      veg:SolitaryVegetationObject ;
        rdfs:label       "species"@en ;
        rdfs:range       iso19136:Code ;
        skos:definition  "SIG3D: Botanical classification of the SolitaryVegetationObject"@en ;
        skos:prefLabel   "species"@en .

veg:SolitaryVegetationObject.lod3Geometry
        a                owl:ObjectProperty ;
        rdfs:domain      veg:SolitaryVegetationObject ;
        rdfs:label       "lod3Geometry"@en ;
        rdfs:range       gsp:Geometry ;
        skos:definition  "SIG3D: Relation to LOD3 geometry of SolitaryVegetationObject.The LOD concept for the module Vegetation is defined in chapter ..."@en ;
        skos:prefLabel   "lod3Geometry"@en .

veg:SolitaryVegetationObject.class
        a                owl:ObjectProperty ;
        rdfs:domain      veg:SolitaryVegetationObject ;
        rdfs:label       "class"@en ;
        rdfs:range       iso19136:Code ;
        skos:definition  "SIG3D: Classification of SolitaryVegetationObject as given by the relevant national regulations, information communities, or specific applications."@en ;
        skos:prefLabel   "class"@en .

<http://www.opengis.net/citygml/vegetation/2.0/vegetation>
        a               owl:Ontology ;
        rdfs:label      "Vegetation"@en ;
        owl:imports     <http://www.opengis.net/citygml/2.0/core> , <http://www.opengis.net/ont/geosparql> , <http://shapechange.net/resources/ont/base> , <http://def.isotc211.org/iso19150/-2/2012/base> ;
        skos:prefLabel  "Vegetation"@en .

veg:PlantCover.usage  a  owl:ObjectProperty ;
        rdfs:domain      veg:PlantCover ;
        rdfs:label       "usage"@en ;
        rdfs:range       iso19136:Code ;
        skos:definition  "SIG3D: Usage of PlantCover as given by the relevant national regulations, information communities, or specific applications."@en ;
        skos:prefLabel   "usage"@en .

veg:AbstractVegetationObject
        a                      owl:Class ;
        rdfs:label             "AbstractVegetationObject"@en ;
        rdfs:subClassOf        core:AbstractCityObject ;
        iso19150-2:isAbstract  true ;
        skos:definition        "SIG3D: Abstract super class of SolitaryVegetationObject and PlantCover"@en ;
        skos:prefLabel         "AbstractVegetationObject"@en .

veg:SolitaryVegetationObject.usage
        a                owl:ObjectProperty ;
        rdfs:domain      veg:SolitaryVegetationObject ;
        rdfs:label       "usage"@en ;
        rdfs:range       iso19136:Code ;
        skos:definition  "SIG3D: Usage of SolitaryVegetationObject as given by the relevant national regulations, information communities, or specific applications."@en ;
        skos:prefLabel   "usage"@en .

veg:PlantCover.lod1MultiSurface
        a                owl:ObjectProperty ;
        rdfs:domain      veg:PlantCover ;
        rdfs:label       "lod1MultiSurface"@en ;
        rdfs:range       gsp:Geometry ;
        skos:definition  "SIG3D:  Relation to a LOD1 surface geometry of PlantCover.The LOD concept for the module Vegetation is defined in chapter ..."@en ;
        skos:prefLabel   "lod1MultiSurface"@en .

veg:PlantCover.lod2MultiSurface
        a                owl:ObjectProperty ;
        rdfs:domain      veg:PlantCover ;
        rdfs:label       "lod2MultiSurface"@en ;
        rdfs:range       gsp:Geometry ;
        skos:definition  "SIG3D: Relation to a LOD2 surface geometry of PlantCover.The LOD concept for the module Vegetation is defined in chapter ..."@en ;
        skos:prefLabel   "lod2MultiSurface"@en .

veg:SolitaryVegetationObject.lod2Geometry
        a                owl:ObjectProperty ;
        rdfs:domain      veg:SolitaryVegetationObject ;
        rdfs:label       "lod2Geometry"@en ;
        rdfs:range       gsp:Geometry ;
        skos:definition  "SIG3D: Relation to LOD2 geometry of SolitaryVegetationObject.The LOD concept for the module Vegetation is defined in chapter ..."@en ;
        skos:prefLabel   "lod2Geometry"@en .

veg:PlantCover.lod3MultiSurface
        a                owl:ObjectProperty ;
        rdfs:domain      veg:PlantCover ;
        rdfs:label       "lod3MultiSurface"@en ;
        rdfs:range       gsp:Geometry ;
        skos:definition  "SIG3D: Relation to a LOD3 surface geometry of PlantCover.The LOD concept for the module Vegetation is defined in chapter ..."@en ;
        skos:prefLabel   "lod3MultiSurface"@en .

veg:SolitaryVegetationObject.height
        a                owl:DatatypeProperty ;
        rdfs:domain      veg:SolitaryVegetationObject ;
        rdfs:label       "height"@en ;
        rdfs:range       sc:Measure ;
        skos:definition  "SIG3D: Distance between the highest point of the vegetation object and the lowest point of the terrain at the bottom of the object."@en ;
        skos:prefLabel   "height"@en .

veg:SolitaryVegetationObject.function
        a                owl:ObjectProperty ;
        rdfs:domain      veg:SolitaryVegetationObject ;
        rdfs:label       "function"@en ;
        rdfs:range       iso19136:Code ;
        skos:definition  "SIG3D: Function of SolitaryVegetationObject as given by the relevant national regulations, information communities, or specific applications."@en ;
        skos:prefLabel   "function"@en .

veg:SolitaryVegetationObject.crownDiameter
        a                owl:DatatypeProperty ;
        rdfs:domain      veg:SolitaryVegetationObject ;
        rdfs:label       "crownDiameter"@en ;
        rdfs:range       sc:Measure ;
        skos:definition  "SIG3D: Maximal diameter of the crown."@en ;
        skos:prefLabel   "crownDiameter"@en .

veg:SolitaryVegetationObject.trunkDiameter
        a                owl:DatatypeProperty ;
        rdfs:domain      veg:SolitaryVegetationObject ;
        rdfs:label       "trunkDiameter"@en ;
        rdfs:range       sc:Measure ;
        skos:definition  "SIG3D: Value of the trunk's diameter"@en ;
        skos:prefLabel   "trunkDiameter"@en .

veg:PlantCover.lod1MultiSolid
        a                owl:ObjectProperty ;
        rdfs:domain      veg:PlantCover ;
        rdfs:label       "lod1MultiSolid"@en ;
        rdfs:range       gsp:Geometry ;
        skos:definition  "SIG3D: Relation to a LOD1 multiple solid geometry of PlantCover.The LOD concept for the module Vegetation is defined in chapter ..."@en ;
        skos:prefLabel   "lod1MultiSolid"@en .
